src/PL/fol.lean
@@ -1,0 +1,12 @@
+import PL.deduction translation
+
+universes u
+
+namespace pl
+open_locale logic_symbol
+open formula logic
+variables (A : Type u)
+
+
+
+end pl
