src/consistency.lean
@@ -188,8 +188,8 @@ namespace complete
 open Theory
 variables {F} {𝓢 : Type*} [has_finite_character F] [semantics F 𝓢] [complete F 𝓢] {S : 𝓢}
 
-/-
-theorem compactness {T : Theory F} :
+
+theorem compactness [semantics.nontrivial F 𝓢] {T : Theory F} :
   semantics.Satisfiable 𝓢 T ↔ (∀ u ⊆ T, u.finite → semantics.Satisfiable 𝓢 (u : set F)) :=
 ⟨by rintros ⟨S, hS⟩ u ss hu; refine ⟨S, semantics.models_of_ss ss hS⟩,
   begin
@@ -200,10 +200,9 @@ theorem compactness {T : Theory F} :
     exact consistent_iff_Satisfiable.mp this
   end⟩
 
-theorem compactness' {T : Theory F} :
+theorem compactness' [semantics.nontrivial F 𝓢] {T : Theory F} :
   ¬semantics.Satisfiable 𝓢 T ↔ (∃ u ⊆ T, u.finite ∧ ¬semantics.Satisfiable 𝓢 (u : set F)) :=
 by rw[compactness]; simp
--/
 
 end complete
 
